Add model and specs for atomic library

src/goose_lang/lib/atomic/impl.v
@@ -1,24 +1,25 @@
-From Perennial.goose_lang Require Import notation.
+From Perennial.goose_lang Require Import notation typing typed_mem.impl.
 
 (* this code is intended to be used qualified with the atomic module *)
 Module atomic.
 Section goose_lang.
-Context {ext:ffi_syntax}.
+Context {ext:ffi_syntax} {ext_ty: ext_types ext}.
 
-Definition LoadUint64 : val :=
-  λ: "l", Load "l".
+(* these are not values so that they are Atomic *)
 
-Definition LoadUint32 : val := LoadUint64.
+Definition LoadUint64 : expr → expr := Load.
+Definition LoadUint32 : expr → expr := LoadUint64.
+Definition StoreUint64 : expr → expr → expr := AtomicStore.
+Definition StoreUint32 : expr → expr → expr := StoreUint64.
+Definition CompareAndSwapUint64 : expr → expr → expr → expr := CmpXchg.
+Definition CompareAndSwapUint32 : expr → expr → expr → expr := CompareAndSwapUint64.
 
-Definition StoreUint64 : val :=
-  λ: "l" "x", AtomicStore "l" "x".
-
-Definition StoreUint32 : val := StoreUint64.
-
-Definition CompareAndSwapUint64 : val :=
-  λ: "l" "old" "new", CmpXchg "l" "old" "new".
-
-Definition CompareAndSwapUint32 : val := CompareAndSwapUint64.
+(* the type arguments to these functions are passed since that's the GooseLang
+calling convention. They are not needed in the model, since these operations
+only load pointers, and we don't need to know what the shape of the referenced
+data is to write the model. *)
+Definition Pointer__Load (_: ty) : expr → expr := Load.
+Definition Pointer__Store (_: ty) : expr → expr → expr := AtomicStore.
 
 End goose_lang.
 End atomic.
